Deploying to gh-pages from @ xubaiw/reservoir-index@5304d5f9d054bc606c13fada32501b690cd76b3b 🚀

git/marcusrossel/reactor-model/src/ReactorModel/Components/Get.lean
@@ -1,4 +1,4 @@
-import ReactorModel.Components.Reactor.Properties
+import ReactorModel.Components.Reactor.Basic
 
 open Classical 
 
@@ -61,10 +61,10 @@ def cmp {σ i} : (cmp : Cmp) → (h : i ∈ (σ.cmp cmp).ids) → Lineage σ i
 -- This function returns that reactor along with its ID.
 -- If the direct parent is the top-level reactor `σ`, then the ID is `⊤`.
 def parent {σ i} : Lineage σ i → (Rooted ID × Reactor)
-  | @nest _ σ' _ i' n _ => 
-    match n with 
-    | nest .. => parent n 
-    | _ => (i', σ')
+  | @nest _ _ r j l _ => 
+    match l with 
+    | nest .. => parent l
+    | _ => (j, r)
   | _ => (⊤, σ)
 
 @[simp] theorem cmp_parent {σ i cmp} (h : i ∈ (σ.cmp cmp).ids) : (Lineage.cmp cmp h).parent.snd = σ := by
@@ -209,5 +209,15 @@ theorem ids_def {σ : Reactor} {cmp : Cmp} {i : ID} :
     simp only [ids, Set.finite.mem_to_finset] at *
     exact h
   )
+
+noncomputable def allIDs (σ : Reactor) : Finset ID :=
+  let description := { i : ID | ∃ cmp, i ∈ σ.ids cmp }
+  let finite : description.finite := sorry
+  finite.toFinset
+
+theorem Object.ext {σ₁ σ₂ : Reactor} (hi : σ₁.allIDs = σ₂.allIDs) (hv : ∀ cmp i v, σ₁ *[cmp:i]= v → σ₂ *[cmp:i]= v) : 
+  σ₁ = σ₂ := by
+    sorry
+
 
 end Reactor
