git/FWuermse/lean-postgres/Postgres/Response.lean
@@ -1,22 +1,121 @@
-class FromByteArray (α : Type u) where
-  fromByteArray? : Section → Except String α
+/-
+  Copyright (c) 2022 Florian Würmseer. All rights reserved.
+  Released under Apache 2.0 license as described in the file LICENSE.
+  Authors: Florian Würmseer
+-/
 
-export FromByteArray (fromByteArray?)
+import Socket
+import Postgres.Util
 
-structure Column where
+open Socket
+open Util
+open List (map foldr range)
+open ByteArray
+open Prod (fst snd)
+
+structure Field where
   length : UInt32
   data : String
+
+instance : ToString Field where
+  toString s := s.data
+
+structure Column where
+  colName: String
+  tableOID: UInt32
+  colIndex: UInt16
+  typeOID: UInt32
+  colLength: UInt16
+  typeModifyer: UInt32
+  format: UInt16
+
+instance : ToString Column where
+  toString c := c.colName
 
 structure RowDescription where
   method : Char
   length : UInt32
+  columnCount : UInt16
+  columns : List Column
+
+instance : ToString RowDescription where
+  toString rd := " × ".intercalate (map toString rd.columns)
+
+structure DataRow where
+  method : Char
+  length : UInt32
   fieldCount : UInt16
-  fields : List String
+  fields : List Field
 
-inductive DataRow where
-  | none
-  | some : Char → UInt32 → UInt16 → List Column → DataRow → DataRow
+instance : ToString DataRow where
+  toString dr := "(" ++ ", ".intercalate (map toString dr.fields) ++ ")"
 
-inductive Section where
-  | rowDesc : RowDescription → Section
-  | dataRow : DataRow → Section
+structure Section where
+  rowDesc : RowDescription
+  dataRow : List DataRow
+
+instance : ToString Section where
+  toString s := s!"{s.rowDesc}\n" ++ "\n".intercalate (map toString s.dataRow)
+
+namespace QueryResponse
+
+def parseColumn (bs : ByteArray) : Column × ByteArray :=
+  let (colName, rest) := takeString bs
+  let (tableOID, rest) := take4 rest
+  let (colIndex, rest) := take2 rest
+  let (typeOID, rest) := take4 rest
+  let (colLength, rest) := take2 rest
+  let (typeModifyer, rest) := take4 rest
+  let (format, rest) := take2 rest
+  (⟨
+    colName,
+    tableOID,
+    colIndex,
+    typeOID,
+    colLength,
+    typeModifyer,
+    format
+  ⟩, rest)
+
+/--
+  Parses `n` elements `α` recursively with the given parse function `parseα`
+-/
+partial def parse {α : Type u} : UInt16 → Option (List α) → (ByteArray → α × ByteArray) → ByteArray → List α × ByteArray
+  | 0, some xs, _, ba => (xs, ba)
+  | n, none, parseα, ba => parse (n-1) (some [fst $ parseα ba]) parseα (snd $ parseα ba)
+  | n, some xs, parseα, ba => parse (n-1) (some $ xs.append [fst $ parseα ba]) parseα (snd $ parseα ba)
+
+def parseField (ba : ByteArray) : Field × ByteArray :=
+  let (length, rest) := take4 ba
+  let (content, rest) := takeNAsStr length.toNat rest
+  (⟨length, content⟩, rest)
+
+partial def parseRows (socket : Socket) (l : List DataRow) : IO $ List DataRow := do
+  let method := Char.ofNat (← socket.recv 1)[0].toNat
+  if method != 'D' then
+    return l
+  let length := toUInt32LE (← socket.recv 4)
+  let fieldCount := toUInt16LE $ ← socket.recv 2
+  -- Excluding 6 Bytes for length and field count
+  let content ← socket.recv (length - 6).toUSize
+  let (fields, _) := parse fieldCount none parseField content
+  parseRows socket (l.append [⟨method, length, fieldCount, fields⟩])
+
+def parseQueryResponse (socket : Socket) : IO Section := do
+  let method := Char.ofNat (← socket.recv 1)[0].toNat
+  let length := toUInt32LE $ ← socket.recv 4
+  let fieldCount := toUInt16LE $ ← socket.recv 2
+  -- Excluding 6 Bytes for length and field count
+  let content ← socket.recv (length - 6).toUSize
+  let (columns, _) := parse fieldCount none parseColumn content
+  pure ⟨
+    ⟨
+      method,
+      length,
+      fieldCount,
+      columns
+    ⟩,
+    (← parseRows socket [])
+  ⟩
+
+end QueryResponse
