git/leanprover/lean4/tests/lean/run/hlistOverload.lean
@@ -1,0 +1,36 @@
+inductive HList : List (Type u) → Type (u+1)
+  | nil  : HList []
+  | cons : α → HList αs → HList (α::αs)
+
+-- Overload `::` notation for HLists
+infix:67 " :: " => HList.cons
+
+-- Overload `[]` notation for HLists
+syntax (name := hlist) "[" term,* "]"  : term
+macro_rules (kind := hlist)
+  | `([ ])           => `(HList.nil)
+  | `([ $a ])        => `(HList.cons $a HList.nil)
+  | `([ $a, $as,* ]) => `(HList.cons $a [$as,*])
+
+def List.nth : (as : List α) → (i : Fin as.length) → α
+  | a::as, ⟨0, _⟩   => a
+  | a::as, ⟨i+1, h⟩ => nth as ⟨i, Nat.lt_of_succ_lt_succ h⟩
+
+def HList.nth : HList αs → (n : Fin αs.length) → αs.nth n
+  | x::_,  ⟨0, _⟩   => x
+  | _::xs, ⟨n+1, h⟩ => xs.nth ⟨n, Nat.lt_of_succ_lt_succ h⟩
+
+def HList.length : HList αs → Nat
+  | []    => 0
+  | _::xs => xs.length
+
+-- Helper notation for creating Fin literals
+notation:max "#" a:max  => (Fin.mk a (by decide))
+
+example : [10, true, 20.1].nth #0 = (10:Nat) := rfl
+example : [10, true, 20.1].nth #1 = true     := rfl
+example : [10, true, 20.1].nth #2 = 20.1     := rfl
+
+#eval [10, true, 20.1].nth #0
+#eval [10, true, 20.1].nth #1
+#eval [10, true, 20.1].nth #2
