git/marcusrossel/reactor-model/src/ReactorModel/Components/Reaction.lean
@@ -2,7 +2,11 @@ import ReactorModel.Components.Change
 
 open Port Classical
 
-open Reaction
+structure Reaction.Input where
+  portVals : ID ▸ Value
+  acts : ID ▸ Value
+  state : ID ▸ Value
+  time : Time.Tag
 
 -- Reactions are the components that can produce changes in a reactor system.
 -- The can be classified into "normal" reactions and "mutations". The `Reaction`
@@ -15,27 +19,25 @@ open Reaction
 -- This field is used to define when a reaction triggers (cf. `triggersOn`).
 --
 -- The `outDepOnly` represents a constraint on the reaction's `body`.
---
--- The `children` are a concept that only applies to mutations. When mutations
--- produce a `Change.create <reactor> <id>`, they need to remember the `<id>`
--- of the reactor they created (for reasons that are related to the execution model). 
--- These IDs are recorded in their `children` field. Since "normal" reactions can't 
--- create reactors (since this is a mutating change), they can't have children. 
--- This is enforced by `normNoChild` (the condition `∀ i s c, c ∈ (body i s) → ¬c.mutates` 
--- is precisely the definition of `isNorm`, but we couldn't use `isNorm` in the definition 
--- of `Reaction` yet, as this would be circular).
-@[ext]
-structure Reaction where
+open Reaction in
+@[ext] structure Reaction where
   deps :          Port.Role → Finset ID
   triggers :      Finset ID
   prio :          Priority
   body :          Input → List Change
   tsSubInDeps :   triggers ⊆ deps Role.in
-  prtOutDepOnly : ∀ i {o} (v : Value),     (o ∉ deps Role.out) → Change.port o v ∉ body i
-  actOutDepOnly : ∀ i {o} (t) (v : Value), (o ∉ deps Role.out) → Change.action o t v ∉ body i
-  actNotPast :    ∀ i a t (v : Value), (Change.action a t v) ∈ body i → i.time.t ≤ t
+  prtOutDepOnly : ∀ i {o} v,   (o ∉ deps Role.out) → Change.port o v ∉ body i
+  actOutDepOnly : ∀ i {o} t v, (o ∉ deps Role.out) → Change.action o t v ∉ body i
+  actNotPast :    ∀ {i a t v}, (Change.action a t v) ∈ body i → i.time.t ≤ t
   
 namespace Reaction
+
+structure Isomorphism (rcn₁ rcn₂ : Reaction) (iso : ID → ID) : Prop where
+  bij :      Function.bijective iso
+  deps :     ∀ r, rcn₁.deps r = (rcn₂.deps r).image map
+  triggers : rcn₁.triggers = rcn₂.triggers.image map
+  prio :     rcn₁.prio = rcn₂.prio
+  body :     ∀ i, List.forall₂ (·.image iso = ·) (rcn₁.body i) (rcn₂.body i)
 
 -- A coercion so that reactions can be called directly as functions.
 -- So when you see something like `rcn p s` that's the same as `rcn.body p s`.
@@ -52,7 +54,7 @@ def isMut (rcn : Reaction) : Prop := ¬rcn.isNorm
 
 -- A reaction is pure if it does not interact with its parent reactor's state.
 structure isPure (rcn : Reaction) : Prop where
-  input : ∀ p a s₁ s₂ t, rcn ⟨p, a, s₁, t⟩ = rcn ⟨p, a, s₂, t⟩ 
+  input : ∀ i s, rcn i = rcn { i with state := s }
   output : ∀ i c, c ∈ rcn.body i → ∃ p v, c = Change.port p v
 
 theorem muts_not_pure (rcn : Reaction) : rcn.isMut → ¬rcn.isPure := by
