git/yatima-inc/Http.lean/src/Http/URI.lean
@@ -1,0 +1,121 @@
+import Std
+import Http.Parsec
+import Http.Types
+import Socket
+
+open Std Parsec Socket
+
+namespace Http
+
+namespace URI
+
+private def toString (uri : URI) : String :=
+  s!"{uri.scheme}://"
+  ++ if let some user := uri.userInfo then s!"{user}@"
+  else ""
+  ++ s!"{uri.host}"
+  ++ if let some port := uri.port then s!":{port}"
+  else ""
+  ++ s!"{uri.path}"
+  ++ if let some query := uri.query then s!"?{query}"
+  else ""
+  ++ if let some fragment := uri.fragment then s!"#{fragment}"
+  else ""
+
+instance : ToString URI := ⟨toString⟩
+
+namespace Parser
+
+def schemeParser : Parsec Scheme :=
+  Scheme.mk <$> manyChars (asciiLetter <|> oneOf ['+', '-', '.'])
+
+def hostName : Parsec Hostname := do
+  let name := many1Chars (asciiLetter <|> digit <|> pchar '-')
+  let start := name ++ pstring "."
+  many1Strings start ++ name
+
+def parseDigit! (c : Char) : Nat :=
+  match c with
+  | '0' => 0
+  | '1' => 1
+  | '2' => 2
+  | '3' => 3
+  | '4' => 4
+  | '5' => 5
+  | '6' => 6
+  | '7' => 7
+  | '8' => 8
+  | '9' => 9
+  | _ => panic! "Not a digit"
+
+def parseUInt16 : Parsec UInt16 := do
+  let as ← many1 digit
+  let mut n := 0
+  for (i, c) in as.toList.reverse.enum do
+    let d := parseDigit! c
+    n := n + d * 10 ^ i
+  return n.toUInt16
+
+def maybePort : Parsec (Option UInt16) := do
+  option $ parseUInt16
+
+def psegment : Parsec String :=
+  many1Chars <| oneOf ['-', '%', '_', '+', '$', '.', ':', '*', '@' ] <|> asciiLetter <|> digit
+
+partial def pathParser : Parsec Path := do
+  let rec comp : Parsec Path := do
+    if ← test <| pstring "/" then
+      let part ← psegment
+      let rest ← comp
+      pure <| part :: rest
+    else
+      pure []
+  comp
+
+def userInfoParser : Parsec UserInfo := do
+  let username ← many1Chars <| asciiLetter <|> digit
+  let password ← option do skipChar ':'; many1Chars <| asciiLetter <|> digit
+  skipChar '@'
+  return { username, password : UserInfo }
+
+partial def queryParser : Parsec Query := do
+  skipChar '?'
+  let rec entries := do
+    let k ← psegment
+    skipChar '='
+    let v ← psegment
+    if ← test $ skipChar '&' then
+      pure <| (k, v) :: (← entries)
+    else
+      pure [(k, v)]
+  entries
+
+partial def fragmentParser : Parsec Fragment := do
+  skipChar '#'
+  let rec entries := do
+    let k ← psegment
+    skipChar '='
+    let v ← psegment
+    if ← test $ skipChar '&' then
+      pure <| (k, v) :: (← entries)
+    else
+      pure [(k, v)]
+  entries
+
+def url : Parsec URI := do  
+  let scheme ← schemeParser
+  skipString "://"
+  let userInfo ← option userInfoParser
+  let host ← hostName
+  let optPort ← maybePort
+  let path ← pathParser
+  let query ← option queryParser
+  let fragment ← option fragmentParser
+  return { scheme, host, port := optPort, path, query, fragment, userInfo : URI }
+
+end Parser
+
+def parse (s : String) : Except String URI := Parser.url.parse s
+
+end URI
+end Http
